lib_avl_mono/Impl.Trees.Types.fst
@@ -11,7 +11,6 @@ module US = FStar.SizeT
 module U64 = FStar.UInt64
 module U32 = FStar.UInt32
 module U8 = FStar.UInt8
-module I64 = FStar.Int64
 
 noextract inline_for_extraction
 let array = Steel.ST.Array.array
@@ -20,13 +19,22 @@ open Constants
 open Config
 open Utils2
 
-// this is a compilation-time assert, see c/utils.c static_assert usage
-assume val avl_data_size_aux : v:U32.t{U32.v v <= 64}
-
-let avl_data_size : v:sc{U32.v avl_data_size_aux <= U32.v v} = 64ul
-
 open SizeClass
 open Main
+
+open Impl.Trees.Cast.M
+
+inline_for_extraction noextract
+let data = data
+
+inline_for_extraction noextract
+let node = node
+
+inline_for_extraction noextract
+let cmp = cmp
+
+inline_for_extraction noextract
+let avl_data_size = avl_data_size
 
 inline_for_extraction noextract
 val init_avl_scs (slab_region: array U8.t)
@@ -97,73 +105,7 @@ let metadata_slabs : mmap_md_slabs = init_mmap_md_slabs ()
 
 #restart-solver
 
-type data = x: (array U8.t * US.t){
-  (
-    US.v (snd x) > 0 /\
-    US.v (snd x) > U32.v page_size /\
-    A.length (fst x) == US.v (snd x) /\
-    A.is_full_array (fst x)
-  )
-  \/
-  US.v (snd x) == 0
-}
-
-let node = node data
-
 module G = FStar.Ghost
-
-assume val ref_node__to__array_u8_tot
-  (x: ref node)
-  : Pure (G.erased (array U8.t))
-  (requires not (is_null x))
-  (ensures fun r ->
-    not (A.is_null (G.reveal r)) /\
-    A.length (G.reveal r) == U32.v avl_data_size
-  )
-
-assume val ref_node__to__array_u8
-  (x: ref node)
-  : Steel (array U8.t)
-  (vptr x)
-  (fun r -> A.varray r)
-  (requires fun _ -> not (is_null x))
-  (ensures fun _ r _ ->
-    not (is_null x) /\
-    not (A.is_null r) /\
-    A.length r == U32.v avl_data_size /\
-    r == G.reveal (ref_node__to__array_u8_tot x)
-  )
-
-assume val array_u8__to__ref_node_tot
-  (arr: array U8.t)
-  : Pure (G.erased (ref node))
-  (requires A.length arr == U32.v avl_data_size)
-  (ensures fun r ->
-    not (is_null (G.reveal r))
-  )
-
-assume val array_u8__to__ref_node
-  (arr: array U8.t)
-  : Steel (ref node)
-  (A.varray arr)
-  (fun r -> vptr r)
-  (requires fun _ -> A.length arr == U32.v avl_data_size)
-  (ensures fun _ r _ ->
-    not (is_null r) /\
-    A.length arr == U32.v avl_data_size /\
-    r == G.reveal (array_u8__to__ref_node_tot arr)
-  )
-
-//CAUTION
-assume val array_u8__to__ref_node_bijectivity
-  (ptr: array U8.t)
-  : Lemma
-  (requires A.length ptr == U32.v avl_data_size)
-  (ensures (
-    let x_cast1 = G.reveal (array_u8__to__ref_node_tot ptr) in
-    let x_cast2 = G.reveal (ref_node__to__array_u8_tot x_cast1) in
-    ptr == x_cast2
-  ))
 
 module UP = FStar.PtrdiffT
 
@@ -173,7 +115,7 @@ let p : hpred data
   G.hide (fun (x: ref node) ->
     is_null x \/
     (not (is_null x) /\
-      (let ptr = ref_node__to__array_u8_tot x in
+      (let ptr = Impl.Trees.Cast.M.ref_node__to__array_u8_tot x in
       same_base_array ptr metadata_slabs.scs.slab_region /\
       UP.fits (A.offset (A.ptr_of ptr) - A.offset (A.ptr_of metadata_slabs.scs.slab_region)) /\
       A.offset (A.ptr_of ptr) - A.offset (A.ptr_of metadata_slabs.scs.slab_region) >= 0 /\
@@ -183,19 +125,6 @@ let p : hpred data
 #pop-options
 
 let t = x:(t data){(G.reveal p) x}
-
-// CAUTION:
-// the refinement implies that the injectivity
-// of the cast uint8_t* -> uintptr_t
-// over:
-// - valid pointers of large allocations
-// (that is the set contained by the AVL tree)
-// - those supplied by the user to free and realloc functions
-// is part of the model
-assume val cmp
-  : f:Impl.Common.cmp data{
-    forall (x y: data). I64.v (f x y) == 0 ==> fst x == fst y
-  }
 
 unfold type f_malloc
   = (x: node) -> Steel (ref node)
