lib_avl_mono/Impl.Trees.Cast.M.fst
@@ -1,0 +1,104 @@
+module Impl.Trees.Cast.M
+
+module US = FStar.SizeT
+module U32 = FStar.UInt32
+module U8 = FStar.UInt8
+module I64 = FStar.Int64
+
+module R = Steel.Reference
+module A = Steel.Array
+open Steel.Effect.Atomic
+open Steel.Effect
+
+module G = FStar.Ghost
+
+open Constants
+open Utils2
+
+// this is a compilation-time assert, see c/utils.c static_assert usage
+assume val avl_data_size_aux : v:U32.t{U32.v v <= 64}
+
+let avl_data_size : v:sc{U32.v avl_data_size_aux <= U32.v v} = 64ul
+
+type data = x: (array U8.t * US.t){
+  (
+    US.v (snd x) > 0 /\
+    US.v (snd x) > U32.v page_size /\
+    A.length (fst x) == US.v (snd x) /\
+    A.is_full_array (fst x)
+  )
+  \/
+  US.v (snd x) == 0
+}
+
+open Impl.Core
+let node = node data
+
+// CAUTION:
+// the refinement implies that the injectivity
+// of the cast uint8_t* -> uintptr_t
+// over:
+// - valid pointers of large allocations
+// (that is the set contained by the AVL tree)
+// - those supplied by the user to free and realloc functions
+// is part of the model
+assume val cmp
+  : f:Impl.Common.cmp data{
+    forall (x y: data). I64.v (f x y) == 0 ==> fst x == fst y
+  }
+
+
+
+
+assume val ref_node__to__array_u8_tot
+  (x: R.ref node)
+  : Pure (G.erased (array U8.t))
+  (requires not (R.is_null x))
+  (ensures fun r ->
+    not (A.is_null (G.reveal r)) /\
+    A.length (G.reveal r) == U32.v avl_data_size
+  )
+
+assume val ref_node__to__array_u8
+  (x: R.ref node)
+  : Steel (array U8.t)
+  (R.vptr x)
+  (fun r -> A.varray r)
+  (requires fun _ -> not (R.is_null x))
+  (ensures fun _ r _ ->
+    not (R.is_null x) /\
+    not (A.is_null r) /\
+    A.length r == U32.v avl_data_size /\
+    r == G.reveal (ref_node__to__array_u8_tot x)
+  )
+
+assume val array_u8__to__ref_node_tot
+  (arr: array U8.t)
+  : Pure (G.erased (R.ref node))
+  (requires A.length arr == U32.v avl_data_size)
+  (ensures fun r ->
+    not (R.is_null (G.reveal r))
+  )
+
+assume val array_u8__to__ref_node
+  (arr: array U8.t)
+  : Steel (R.ref node)
+  (A.varray arr)
+  (fun r -> R.vptr r)
+  (requires fun _ -> A.length arr == U32.v avl_data_size)
+  (ensures fun _ r _ ->
+    not (R.is_null r) /\
+    A.length arr == U32.v avl_data_size /\
+    r == G.reveal (array_u8__to__ref_node_tot arr)
+  )
+
+//CAUTION
+assume val array_u8__to__ref_node_bijectivity
+  (ptr: array U8.t)
+  : Lemma
+  (requires A.length ptr == U32.v avl_data_size)
+  (ensures (
+    let x_cast1 = G.reveal (array_u8__to__ref_node_tot ptr) in
+    let x_cast2 = G.reveal (ref_node__to__array_u8_tot x_cast1) in
+    ptr == x_cast2
+  ))
